Replace Loc with FLoc

src/lang/Memory.v
@@ -7,6 +7,8 @@ Require Import Axioms.
 Require Import Basic.
 Require Import DataStructure.
 Require Import DenseOrder.
+Require Import Loc.
+
 Require Import Event.
 Require Import Time.
 Require Import View.
@@ -16,9 +18,9 @@ Set Implicit Arguments.
 
 
 Module Memory.
-  Definition t := Loc.t -> Cell.t.
+  Definition t := FLoc.t -> Cell.t.
 
-  Definition get (loc:Loc.t) (ts:Time.t) (mem:t): option (Time.t * Message.t) :=
+  Definition get (loc:FLoc.t) (ts:Time.t) (mem:t): option (Time.t * Message.t) :=
     Cell.get ts (mem loc).
 
   Lemma get_disjoint
@@ -40,7 +42,7 @@ Module Memory.
         (EXT: forall loc ts, get loc ts lhs = get loc ts rhs):
     lhs = rhs.
   Proof.
-    apply LocFun.ext. i.
+    apply FLocFun.ext. i.
     apply Cell.ext. i.
     apply EXT.
   Qed.
@@ -139,10 +141,10 @@ Module Memory.
   Proof. ii. apply bot_get. Qed.
 
   Definition singleton
-             (loc:Loc.t) (from to:Time.t) (msg:Message.t)
+             (loc:FLoc.t) (from to:Time.t) (msg:Message.t)
              (LT: Time.lt from to)
              (WF: Message.wf msg): t :=
-    (LocFun.add loc (Cell.singleton LT WF)
+    (FLocFun.add loc (Cell.singleton LT WF)
                 (fun _ => Cell.bot)).
 
   Lemma singleton_get
@@ -150,13 +152,13 @@ Module Memory.
         (LT:Time.lt from to)
         (WF: Message.wf msg):
     get l t (singleton loc LT WF) =
-    if Loc.eq_dec l loc
+    if FLoc.eq_dec l loc
     then if Time.eq_dec t to
          then Some (from, msg)
          else None
     else None.
   Proof.
-    unfold get, singleton. unfold LocFun.add, LocFun.find.
+    unfold get, singleton. unfold FLocFun.add, FLocFun.find.
     repeat condtac; subst.
     - rewrite Cell.singleton_get. condtac; [|congr]. auto.
     - rewrite Cell.singleton_get. condtac; [congr|]. auto.
@@ -165,7 +167,7 @@ Module Memory.
 
   Definition init: t := fun _ => Cell.init.
 
-  Fixpoint domain (locs: list Loc.t) (mem: t): list (Loc.t * Time.t) :=
+  Fixpoint domain (locs: list FLoc.t) (mem: t): list (FLoc.t * Time.t) :=
     match locs with
     | [] => []
     | hd::tl =>
@@ -179,7 +181,7 @@ Module Memory.
     forall loc from to msg (GET: get loc to mem = Some (from, msg)),
       List.In (loc, to) dom.
   Proof.
-    destruct Loc.finite.
+    destruct FLoc.finite.
     exists (domain x mem). i. specialize (H loc).
     revert H from to msg GET.
     induction x; ss; i. des.
@@ -190,7 +192,7 @@ Module Memory.
     - apply List.in_or_app. right. eauto.
   Qed.
 
-  Inductive message_to: forall (msg:Message.t) (loc:Loc.t) (to:Time.t), Prop :=
+  Inductive message_to: forall (msg:Message.t) (loc:FLoc.t) (to:Time.t), Prop :=
   | message_to_full
       val released loc to
       (TS: Time.le (released.(View.unwrap).(View.rlx) loc) to):
@@ -278,35 +280,35 @@ Module Memory.
     splits; try econs; ss. refl.
   Qed.
 
-  Inductive add (mem1:t) (loc:Loc.t) (from to:Time.t) (msg:Message.t) (mem2:t): Prop :=
+  Inductive add (mem1:t) (loc:FLoc.t) (from to:Time.t) (msg:Message.t) (mem2:t): Prop :=
   | add_intro
       r
       (ADD: Cell.add (mem1 loc) from to msg r)
-      (MEM2: mem2 = LocFun.add loc r mem1)
+      (MEM2: mem2 = FLocFun.add loc r mem1)
   .
   Hint Constructors add.
 
-  Inductive split (mem1:t) (loc:Loc.t) (ts1 ts2 ts3:Time.t) (msg2 msg3:Message.t) (mem2:t): Prop :=
+  Inductive split (mem1:t) (loc:FLoc.t) (ts1 ts2 ts3:Time.t) (msg2 msg3:Message.t) (mem2:t): Prop :=
   | split_intro
       r
       (SPLIT: Cell.split (mem1 loc) ts1 ts2 ts3 msg2 msg3 r)
-      (MEM2: mem2 = LocFun.add loc r mem1)
+      (MEM2: mem2 = FLocFun.add loc r mem1)
   .
   Hint Constructors split.
 
-  Inductive lower (mem1:t) (loc:Loc.t) (from to:Time.t) (msg1 msg2:Message.t) (mem2:t): Prop :=
+  Inductive lower (mem1:t) (loc:FLoc.t) (from to:Time.t) (msg1 msg2:Message.t) (mem2:t): Prop :=
   | lower_intro
       r
       (LOWER: Cell.lower (mem1 loc) from to msg1 msg2 r)
-      (MEM2: mem2 = LocFun.add loc r mem1)
+      (MEM2: mem2 = FLocFun.add loc r mem1)
   .
   Hint Constructors lower.
 
-  Inductive remove (mem1:t) (loc:Loc.t) (from1 to1:Time.t) (msg1:Message.t) (mem2:t): Prop :=
+  Inductive remove (mem1:t) (loc:FLoc.t) (from1 to1:Time.t) (msg1:Message.t) (mem2:t): Prop :=
   | remove_intro
       r
       (REMOVE: Cell.remove (mem1 loc) from1 to1 msg1 r)
-      (MEM2: mem2 = LocFun.add loc r mem1)
+      (MEM2: mem2 = FLocFun.add loc r mem1)
   .
   Hint Constructors remove.
 
@@ -378,7 +380,7 @@ Module Memory.
 
   Inductive promise
             (promises1 mem1:t)
-            (loc:Loc.t) (from to:Time.t) (msg:Message.t)
+            (loc:FLoc.t) (from to:Time.t) (msg:Message.t)
             (promises2 mem2:t): forall (kind:op_kind), Prop :=
   | promise_add
       (PROMISES: add promises1 loc from to msg promises2)
@@ -410,7 +412,7 @@ Module Memory.
 
   Inductive write
             (promises1 mem1:t)
-            (loc:Loc.t) (from1 to1:Time.t) (val:Const.t) (released: option View.t)
+            (loc:FLoc.t) (from1 to1:Time.t) (val:Const.t) (released: option View.t)
             (promises3 mem2:t) (kind:op_kind): Prop :=
   | write_intro
       promises2
@@ -431,7 +433,7 @@ Module Memory.
     then Some (from, msg)
     else get l t mem1.
   Proof.
-    inv ADD. unfold get, LocFun.add. condtac.
+    inv ADD. unfold get, FLocFun.add. condtac.
     - subst. erewrite Cell.add_o; eauto.
       repeat (condtac; subst; des; ss; try congr).
     - repeat (condtac; subst; des; ss; try congr).
@@ -448,7 +450,7 @@ Module Memory.
          then Some (ts2, msg3)
          else get l t mem1.
   Proof.
-    inv SPLIT. unfold get, LocFun.add. condtac.
+    inv SPLIT. unfold get, FLocFun.add. condtac.
     - subst. erewrite Cell.split_o; eauto.
       repeat (condtac; subst; des; ss; try congr).
     - repeat (condtac; subst; des; ss; try congr).
@@ -463,7 +465,7 @@ Module Memory.
     then Some (from, msg2)
     else get l t mem1.
   Proof.
-    inv LOWER. unfold get, LocFun.add. condtac.
+    inv LOWER. unfold get, FLocFun.add. condtac.
     - subst. erewrite Cell.lower_o; eauto.
       repeat (condtac; subst; des; ss; try congr).
     - repeat (condtac; subst; des; ss; try congr).
@@ -478,7 +480,7 @@ Module Memory.
     then None
     else get l t mem1.
   Proof.
-    inv REMOVE. unfold get, LocFun.add. condtac.
+    inv REMOVE. unfold get, FLocFun.add. condtac.
     - subst. erewrite Cell.remove_o; eauto.
       repeat (condtac; subst; des; ss; try congr).
     - repeat (condtac; subst; des; ss; try congr).
@@ -491,7 +493,7 @@ Module Memory.
     <<GET: get loc to1 mem2 = Some (from1, msg1)>>.
   Proof.
     inv ADD. eapply Cell.add_get0; eauto.
-    unfold get, Cell.get, LocFun.add. condtac; ss.
+    unfold get, Cell.get, FLocFun.add. condtac; ss.
   Qed.
 
   Lemma split_get0
@@ -503,7 +505,7 @@ Module Memory.
     <<GET: get loc ts3 mem2 = Some (ts2, msg3)>>.
   Proof.
     inv SPLIT. eapply Cell.split_get0; eauto.
-    unfold get, Cell.get, LocFun.add. condtac; ss.
+    unfold get, Cell.get, FLocFun.add. condtac; ss.
   Qed.
 
   Lemma lower_get0
@@ -514,7 +516,7 @@ Module Memory.
     <<MSG_LE: Message.le msg2 msg1>>.
   Proof.
     inv LOWER. eapply Cell.lower_get0; eauto.
-    unfold get, Cell.get, LocFun.add. condtac; ss.
+    unfold get, Cell.get, FLocFun.add. condtac; ss.
   Qed.
 
   Lemma remove_get0
@@ -524,7 +526,7 @@ Module Memory.
     <<GET: get loc to1 mem2 = None>>.
   Proof.
     inv REMOVE. eapply Cell.remove_get0; eauto.
-    unfold get, Cell.get, LocFun.add. condtac; ss.
+    unfold get, Cell.get, FLocFun.add. condtac; ss.
   Qed.
 
   Lemma add_get1
@@ -1121,7 +1123,7 @@ Module Memory.
         (INHABITED: inhabited mem):
     closed_timemap (TimeMap.singleton loc to) mem.
   Proof.
-    unfold TimeMap.singleton, LocFun.add, LocFun.find. ii. condtac.
+    unfold TimeMap.singleton, FLocFun.add, FLocFun.find. ii. condtac.
     - subst. eauto.
     - apply closed_timemap_bot. auto.
   Qed.
@@ -1162,7 +1164,7 @@ Module Memory.
 
   (* Lemmas on max_timemap *)
 
-  Definition max_ts (loc:Loc.t) (mem:t): Time.t :=
+  Definition max_ts (loc:FLoc.t) (mem:t): Time.t :=
     Cell.max_ts (mem loc).
 
   Lemma max_ts_spec
@@ -1231,7 +1233,7 @@ Module Memory.
 
   (* Lemmas on max_full_timemap *)
 
-  Definition max_full_ts (mem: t) (loc: Loc.t) (ts: Time.t): Prop :=
+  Definition max_full_ts (mem: t) (loc: FLoc.t) (ts: Time.t): Prop :=
     Cell.max_full_ts (mem loc) ts.
 
   Lemma max_full_ts_exists
@@ -1502,7 +1504,7 @@ Module Memory.
     - eapply lower_max_full_timemap; eauto.
   Qed.
 
-  Inductive max_full_released (mem: t) (loc: Loc.t) (ts: Time.t): forall (released: View.t), Prop :=
+  Inductive max_full_released (mem: t) (loc: FLoc.t) (ts: Time.t): forall (released: View.t), Prop :=
   | max_full_released_intro
       tm rlx
       (MAX: max_full_timemap mem tm)
@@ -1578,11 +1580,11 @@ Module Memory.
       + subst. etrans; [|exact REL_TS].
         inv ADD. inv ADD0. inv MSG_WF. inv WF. apply WF0.
       + etrans; [apply PLN|]. apply Time.join_spec; [refl|].
-        unfold TimeMap.singleton, LocFun.add. condtac; ss. apply Time.bot_spec.
+        unfold TimeMap.singleton, FLocFun.add. condtac; ss. apply Time.bot_spec.
     - ii. unfold TimeMap.add. condtac.
       + subst. ss.
       + etrans; [apply RLX|]. apply Time.join_spec; [refl|].
-        unfold TimeMap.singleton, LocFun.add. condtac; ss. apply Time.bot_spec.
+        unfold TimeMap.singleton, FLocFun.add. condtac; ss. apply Time.bot_spec.
   Qed.
 
   Lemma max_full_released_closed_split
@@ -1624,11 +1626,11 @@ Module Memory.
       + subst. etrans; [|exact REL_TS].
         inv SPLIT. inv SPLIT0. inv MSG_WF. inv WF. apply WF0.
       + etrans; [apply PLN|]. apply Time.join_spec; [refl|].
-        unfold TimeMap.singleton, LocFun.add. condtac; ss. apply Time.bot_spec.
+        unfold TimeMap.singleton, FLocFun.add. condtac; ss. apply Time.bot_spec.
     - ii. unfold TimeMap.add. condtac.
       + subst. ss.
       + etrans; [apply RLX|]. apply Time.join_spec; [refl|].
-        unfold TimeMap.singleton, LocFun.add. condtac; ss. apply Time.bot_spec.
+        unfold TimeMap.singleton, FLocFun.add. condtac; ss. apply Time.bot_spec.
   Qed.
 
   Lemma max_full_released_closed_lower
@@ -1670,11 +1672,11 @@ Module Memory.
       + subst. etrans; [|exact REL_TS].
         inv LOWER. inv LOWER0. inv MSG_WF. inv WF. apply WF0.
       + etrans; [apply PLN|]. apply Time.join_spec; [refl|].
-        unfold TimeMap.singleton, LocFun.add. condtac; ss. apply Time.bot_spec.
+        unfold TimeMap.singleton, FLocFun.add. condtac; ss. apply Time.bot_spec.
     - ii. unfold TimeMap.add. condtac.
       + subst. ss.
       + etrans; [apply RLX|]. apply Time.join_spec; [refl|].
-        unfold TimeMap.singleton, LocFun.add. condtac; ss. apply Time.bot_spec.
+        unfold TimeMap.singleton, FLocFun.add. condtac; ss. apply Time.bot_spec.
   Qed.
 
 
@@ -2128,15 +2130,15 @@ Module Memory.
         (MSG_WF: Message.wf msg):
     remove (singleton loc LT MSG_WF) loc from to msg bot.
   Proof.
-    assert (bot = LocFun.add loc Cell.bot (singleton loc LT MSG_WF)).
+    assert (bot = FLocFun.add loc Cell.bot (singleton loc LT MSG_WF)).
     { apply ext. i. rewrite bot_get.
-      unfold get, LocFun.add, LocFun.find. condtac.
+      unfold get, FLocFun.add, FLocFun.find. condtac.
       - rewrite Cell.bot_get. auto.
-      - unfold singleton, LocFun.add, LocFun.find. condtac; [congr|].
+      - unfold singleton, FLocFun.add, FLocFun.find. condtac; [congr|].
         rewrite Cell.bot_get. auto.
     }
     rewrite H. econs; ss.
-    unfold singleton, LocFun.add, LocFun.find. condtac; [|congr].
+    unfold singleton, FLocFun.add, FLocFun.find. condtac; [|congr].
     eapply Cell.remove_singleton.
   Qed.
 
@@ -2211,7 +2213,7 @@ Module Memory.
     eexists. econs; ss. eauto.
   Qed.
 
-  Definition nonsynch_loc (loc:Loc.t) (mem:t): Prop :=
+  Definition nonsynch_loc (loc:FLoc.t) (mem:t): Prop :=
     forall f t msg (GET: get loc t mem = Some (f, msg)),
       match msg with
       | Message.full _ rel => rel = None
@@ -2326,7 +2328,7 @@ Module Memory.
     exploit Cell.next_exists; eauto.
   Qed.
 
-  Inductive prev (loc: Loc.t) (ts: Time.t) (mem: t) (from to: Time.t) (msg: Message.t): Prop :=
+  Inductive prev (loc: FLoc.t) (ts: Time.t) (mem: t) (from to: Time.t) (msg: Message.t): Prop :=
   | prev_intro
       (GET: get loc to mem = Some (from, msg))
       (TO: Time.le to ts)
@@ -2347,7 +2349,7 @@ Module Memory.
 
   (* adjacent *)
 
-  Inductive adjacent (loc: Loc.t) (from1 to1 from2 to2: Time.t) (mem: t): Prop :=
+  Inductive adjacent (loc: FLoc.t) (from1 to1 from2 to2: Time.t) (mem: t): Prop :=
   | adjacent_intro
       m1 m2
       (GET1: get loc to1 mem = Some (from1, m1))
@@ -2432,7 +2434,7 @@ Module Memory.
 
   (* cap *)
 
-  Inductive latest_val (loc: Loc.t) (mem: t) (val: Const.t): Prop :=
+  Inductive latest_val (loc: FLoc.t) (mem: t) (val: Const.t): Prop :=
   | latest_val_intro
       ts from released
       (MAX: max_full_ts mem loc ts)
@@ -2460,7 +2462,7 @@ Module Memory.
     exists val. econs; eauto.
   Qed.
 
-  Definition latest_half (loc: Loc.t) (promises mem: t): Prop :=
+  Definition latest_half (loc: FLoc.t) (promises mem: t): Prop :=
     match get loc (max_ts loc mem) promises with
     | Some (_, Message.half) => False
     | _ => True
@@ -2716,7 +2718,7 @@ Module Memory.
 
   (* Existence of cap *)
 
-  Inductive cap_imm (loc: Loc.t) (to: Time.t) (view: View.t) (promises mem1 mem2: t): Prop :=
+  Inductive cap_imm (loc: FLoc.t) (to: Time.t) (view: View.t) (promises mem1 mem2: t): Prop :=
   | cap_imm_intro
       (SOUND: forall loc' from' to' msg (GET: get loc' to' mem1 = Some (from', msg)),
           get loc' to' mem2 = Some (from', msg))
@@ -2738,7 +2740,7 @@ Module Memory.
           (from' = max_ts loc mem1 -> latest_half loc promises mem1))
   .
 
-  Inductive cap_aux (dom: list (Loc.t * Time.t)) (view: View.t) (promises mem1 mem2: t): Prop :=
+  Inductive cap_aux (dom: list (FLoc.t * Time.t)) (view: View.t) (promises mem1 mem2: t): Prop :=
   | cap_aux_intro
       (SOUND: forall loc from to msg (GET: get loc to mem1 = Some (from, msg)),
           get loc to mem2 = Some (from, msg))
@@ -3044,7 +3046,7 @@ Module Memory.
     exists mem0. split; auto. unnw. etrans; eauto.
   Qed.
 
-  Fixpoint finite_sound (dom: list (Loc.t * Time.t)) (mem: t): list (Loc.t * Time.t) :=
+  Fixpoint finite_sound (dom: list (FLoc.t * Time.t)) (mem: t): list (FLoc.t * Time.t) :=
     match dom with
     | [] => []
     | (loc, to) :: tl =>
