src/invariant/PFStep.v
@@ -7,6 +7,8 @@ Require Import Axioms.
 Require Import Basic.
 Require Import DataStructure.
 Require Import DenseOrder.
+Require Import Loc.
+
 Require Import Time.
 Require Import Event.
 Require Import Language.
@@ -424,7 +426,7 @@ Module PFStep.
 
   (* existence of sim *)
 
-  Inductive sim_memory_aux (dom: list (Loc.t * Time.t)) (promises mem_src mem_tgt: Memory.t): Prop :=
+  Inductive sim_memory_aux (dom: list (FLoc.t * Time.t)) (promises mem_src mem_tgt: Memory.t): Prop :=
   | sim_memory_aux_intro
       (SOUND: Memory.le mem_src mem_tgt)
       (COMPLETE1: forall loc from to msg
