src/prop/MemoryMerge.v
@@ -8,6 +8,8 @@ Require Import Axioms.
 Require Import Basic.
 Require Import DataStructure.
 Require Import DenseOrder.
+Require Import Loc.
+
 Require Import Event.
 Require Import Time.
 Require Import View.
@@ -25,10 +27,10 @@ Module MemoryMerge.
     Memory.add mem0 loc from to msg2 mem2.
   Proof.
     inv ADD1. inv ADD. inv LOWER2. inv LOWER.
-    rewrite LocFun.add_add_eq. econs; auto.
+    rewrite FLocFun.add_add_eq. econs; auto.
     unfold Cell.add in *.
     destruct r, r0. ss. subst.
-    unfold LocFun.add. condtac; [|congr]. s.
+    unfold FLocFun.add. condtac; [|congr]. s.
     rewrite DOMap.add_add_eq. econs; auto.
   Qed.
 
@@ -39,10 +41,10 @@ Module MemoryMerge.
     Memory.split mem0 loc ts1 ts2 ts3 msg2' msg3 mem2.
   Proof.
     inv SPLIT1. inv SPLIT. inv LOWER2. inv LOWER.
-    rewrite LocFun.add_add_eq. econs; auto.
+    rewrite FLocFun.add_add_eq. econs; auto.
     unfold Cell.split in *.
     destruct r, r0. ss. subst.
-    unfold LocFun.add. condtac; [|congr]. s.
+    unfold FLocFun.add. condtac; [|congr]. s.
     rewrite DOMap.add_add_eq. econs; auto.
   Qed.
 
@@ -53,10 +55,10 @@ Module MemoryMerge.
     Memory.lower mem0 loc from to msg0 msg2 mem2.
   Proof.
     inv LOWER1. inv LOWER. inv LOWER2. inv LOWER.
-    rewrite LocFun.add_add_eq. econs; auto.
+    rewrite FLocFun.add_add_eq. econs; auto.
     unfold Cell.lower in *.
     destruct r, r0. ss. subst.
-    unfold LocFun.add. condtac; [|congr]. s.
+    unfold FLocFun.add. condtac; [|congr]. s.
     rewrite DOMap.add_add_eq. econs; auto.
     etrans; eauto.
   Qed.
